Fixes

Isabelle2/BallotArrays3.thy
@@ -26,9 +26,9 @@ definition conservative_array where
 
 text {* Here the @{term Max} is the one from @{text Lattices_Big} *}
 
-definition proved_safe_at_2_a where
+definition proved_safe_at_abs where
   -- {* Any value that has been proved safe at ballot b can be voted for in ballot b. *}
-  "proved_safe_at_2_a q b v \<equiv>
+  "proved_safe_at_abs q b v \<equiv>
     q \<in> quorums \<and> (\<forall> a \<in> q . ballot a \<ge> b) \<and>
     (if \<exists> a \<in> q . \<exists> b\<^sub>2 . b\<^sub>2 < b \<and> vote a b\<^sub>2 \<noteq> None
     then \<exists> a \<in> q . vote a (Max {b\<^sub>2 . \<exists> a \<in> q . b\<^sub>2 < b \<and> vote a b\<^sub>2 \<noteq> None}) = Some v
