Isabelle2/BallotArrayProperties.thy
@@ -6,7 +6,7 @@ begin
 
 text {* 
 In this theory we show the two main properties of ballot-arrays:
-1) If a value v is @{term "ballot_array.proved_safe_at_2_a q b v"}, then it is @{term "ballot_array.safe_at v b"}}
+1) If a value v is @{term "ballot_array.proved_safe_at_abs q b v"}, then it is @{term "ballot_array.safe_at v b"}}
 2) If a ballot array increases, according to the prefix definition below, then every
 value that was @{term "ballot_array.safe_at v b"} before is still @{term "ballot_array.safe_at v b"}}}
 *}
@@ -84,16 +84,16 @@ qed
 
 text {* The main lemma. Inspired by section 2.2.2 of the paper "Fast Paxos", by Leslie Lamport. *}
 
-lemma proved_safe_at_2_a_imp_safe_at:
+lemma proved_safe_at_abs_imp_safe_at:
   assumes "\<And> a j w . \<lbrakk>j < i; vote a j = Some w\<rbrakk> \<Longrightarrow> safe_at w j"
-  and "proved_safe_at_2_a q i v" and "conservative_array"
+  and "proved_safe_at_abs q i v" and "conservative_array"
   shows "safe_at v (i::nat)"
 proof (cases "i = 0")
   case True thus ?thesis
     by (metis not_less0 safe_at_def)
 next
   case False
-  have "q \<in> quorums" and ballot_q:"\<And> a . a \<in> q \<Longrightarrow> ballot a \<ge> i" using assms(2) by (auto simp add:proved_safe_at_2_a_def)
+  have "q \<in> quorums" and ballot_q:"\<And> a . a \<in> q \<Longrightarrow> ballot a \<ge> i" using assms(2) by (auto simp add:proved_safe_at_abs_def)
   text {* There are two cases: 
     (a) an acceptor a in the quorum q voted in round k < i, 
     and k is the maximum round smaller than i in which an acceptor in q voted;
@@ -111,7 +111,7 @@ next
     def votes \<equiv> "{l . \<exists> a \<in> q . l < i \<and> vote a l \<noteq> None }"
     def k \<equiv> "Max votes"
     from True assms(2) obtain a where "a \<in> q" and "vote a k = Some v"
-      by (auto simp add:proved_safe_at_2_a_def k_def votes_def)
+      by (auto simp add:proved_safe_at_abs_def k_def votes_def)
     moreover have "k < i" and "\<And> a\<^sub>2 l . \<lbrakk>a\<^sub>2 \<in> q; k < l; l < i\<rbrakk> \<Longrightarrow> vote a\<^sub>2 l = None"
     proof -
       have "k \<in> votes" and "\<And> x . x \<in> votes \<Longrightarrow> x \<le> k"
